clean autograder file

state/Examples.Autograder.Old.fst
@@ -28,6 +28,9 @@ let grade_preorder : preorder grade = fun g1 g2 ->
   | NotGraded -> True
   | _ -> g1 == g2
 
+let max_fuel = pow2 32 - 1
+
+(* TODO: two implementations of each : one with Type0 (pred) & one for HO contracts (ST effect) *)
 let rec no_cycles_fuel (fuel:nat) (ll:ref (linkedList 'a)) (h:heap): Type0 =
   match sel h ll with
   | LLNil -> True
@@ -44,25 +47,158 @@ let rec sorted_fuel (fuel:nat) (ll:linkedList int) (h:heap): Type0 =
       | LLNil -> True
       | LLCons y next -> x <= y /\ sorted_fuel (fuel - 1) tl h
 
+let rec footprint_acc
+  (l: linkedList int)
+  (h:heap)
+  (hdom:(FSet.set nat){forall (a:Type) (rel:_) (r:mref a rel). h `contains` r ==> addr_of r `FSet.mem` hdom})
+  (acc:(FSet.set nat){acc `FSet.subset` hdom}) :
+  GTot (FSet.set nat) (decreases (FSet.cardinality (hdom `FSet.difference` acc))) =
+  match l with
+  | LLNil -> acc
+  | LLCons x xsref ->
+    if addr_of xsref `FSet.mem` acc then acc
+    else begin
+      assume (h `contains` xsref); (* Turn this into a type refinement? *)
+      let acc' = (acc `FSet.union` FSet.singleton (addr_of xsref)) in
+      FSet.all_finite_set_facts_lemma ();
+      footprint_acc (sel h xsref) h hdom acc'
+    end
+
+let get_heap_domain h =
+  FSet.all_finite_set_facts_lemma ();
+  let rec aux (n:nat) : res:(FSet.set nat){forall i. 0 < i && i <= n ==> i `FSet.mem` res} =
+    if n = 0 then FSet.emptyset else FSet.singleton n `FSet.union` (aux (n-1)) in
+  aux (next_addr h - 1)
+
+let footprint (l: ref (linkedList int)) (h:heap) : (GTot (FSet.set nat)) =
+  let hdom = get_heap_domain h in
+  FSet.all_finite_set_facts_lemma ();
+  assert (FSet.emptyset `FSet.subset` hdom);
+  assume (forall (a:Type) (rel:_) (r:mref a rel). h `contains` r ==> addr_of r `FSet.mem` hdom);
+  assume (h `contains` l);
+  footprint_acc (sel h l) h hdom (FSet.singleton (addr_of l))
+
+let ll_length (ll: ref (linkedList int)) (h: heap): GTot int =
+  cardinality (footprint ll h)
+
 let no_cycles (ll:ref (linkedList int)) (h:heap): Type0 =
   exists (fuel:nat). no_cycles_fuel fuel ll h
 
 let sorted (ll: ref (linkedList int)) (h:heap): Type0 =
   exists fuel. sorted_fuel fuel (sel h ll) h
 
+let heap_contains_all_refs_of_ll (l: linkedList int) (h: heap): Lemma
+  (requires satisfy_on_heap l h contains_pred)
+  (ensures l == LLNil \/ satisfy_on_heap (sel h (LLCons?.next l)) h contains_pred) = admit()
+
+(* Probably there are built in functions for these in ulib? *)
+let rec search_elem_with_first_comp (v: int) (l: list (int * int)): option (int * int) =
+  match l with
+  | [] -> None
+  | hd::tl ->
+    if fst hd = v then Some hd
+    else search_elem_with_first_comp v tl
+
+let rec elements_of_ll_acc
+  (fuel:nat)
+  (ll:linkedList int)
+  (h:heap)
+  (acc: FSet.set (int * int)) : GTot (FSet.set (int * int)) =
+  if fuel = 0 then acc
+  else
+    match ll with
+    | LLNil -> acc
+    | LLCons v next ->
+        let w = search_elem_with_first_comp v (set_as_list acc) in
+        let acc' =
+        match w with
+        | None -> acc `union` FSet.singleton(v, 1)
+        | Some (v, m) -> ((v, m) `remove` acc) `union` singleton(v, m+1)
+        in let tail = sel h next in
+      elements_of_ll_acc (fuel - 1) tail h acc'
+
+(* let elements_of_ll (fuel: nat) (ll:linkedList int) (h:heap) (acc: FSet.set int) : GTot (FSet.set int) =
+  elements_of_ll_acc fuel ll h FSet.emptyset *) (* Previously: fuel = max_length *)
+
+(**
+let same_elements (ll:ref (linkedList int)) (h0 h1:heap): Type0 =
+  let length_h0 = ll_length ll h0 in
+  let length_h1 = ll_length ll h1 in
+  if length_h0 <> length_h1 then False
+  else
+    exists fuel. elements_of_ll_acc fuel ll h0 FSet.emptyset == elements_of_ll_acc fuel ll h0 FSet.emptyset
+
+let rec no_cycles_SST (fuel: nat) (ll: linkedList int): SST bool
+  (requires fun h0 -> satisfy_on_heap ll h0 contains_pred)
+  (ensures fun h0 r h1 -> h0 == h1 /\ (r ==> no_cycles ll h0)) = (* ==> instead of <==> because this version uses fuel *)
+  if fuel = 0 then false
+  else
+    match ll with
+      | LLNil -> true
+      | LLCons x xsref ->
+        let h0 = get_heap() in
+        assert (h0 `contains` xsref);
+        let tail : linkedList int = sst_read xsref in
+        let h1 = get_heap() in
+        assert (h0 == h1);
+        assume (satisfy_on_heap (sel h0 xsref) h0 contains_pred); (* add lemma for this *)
+        admit(); (* second postcond fails *)
+        no_cycles_SST (fuel - 1) tail
+
+let rec sorted_SST (fuel: nat) (ll: linkedList int): SST bool
+  (requires fun h0 -> satisfy_on_heap ll h0 contains_pred)
+  (ensures fun h0 r h1 -> r ==> sorted ll h0) =
+  if fuel = 0 then false
+  else
+    match ll with
+    | LLNil -> true
+    | LLCons x next ->
+      let tl = sst_read next in
+      match tl with
+      | LLNil -> true
+      | LLCons y next ->
+        if x > y then false
+        else begin
+          let h = get_heap() in
+          heap_contains_all_refs_of_ll ll h;
+          admit();
+          sorted_SST (fuel - 1) tl
+        end
+**)
+// let same_elements_SST (ll: linkedList int): SST bool
+//   (requires fun h0 -> satisfy_on_heap ll h0 contains_pred)
+//   (ensures fun h0 r h1 -> r ==> same_elements ll h0 h1)
+//   = admit()
+
 type student_solution =
-  ll:ref(linkedList int) -> SST (option unit)
+  ll_ref:ref(linkedList int) -> SST (option unit)
     (requires (fun h0 ->
-      h0 `contains` ll /\
-      //no_cycles ll_ref h0 /\
-      is_shared ll h0))
+      //no_cycles (sel h0 ll_ref) h0 /\
+      h0 `contains` ll_ref /\
+      is_shared ll_ref h0))
     (ensures (fun h0 r h1 ->
-      (Some? r ==> no_cycles ll h1 /\ sorted ll h1) /\ // /\ same_elements ll h0 h1) /\
+      (Some? r ==> no_cycles ll_ref h1 /\ sorted ll_ref h1) /\ // /\ same_elements (sel h1 ll_ref) h0 h1) /\
       modifies_only_shared h0 h1 /\
       gets_shared Set.empty h0 h1))
 // let wss : witnessable (list (mref grade grade_preorder * student_solution)) = admit ()
 (*  witnessable_list (witnessable_pair (witnessable_mref witnessable_grade grade_preorder) witnessable_llist) *)
 
+  (**
+let rec no_cycles_acc (l:ref (linkedList int)) (h:heap) (s:set nat) : Type0 =
+  (addr_of l `Set.mem` s ==> False) /\
+  (~(addr_of l `Set.mem` s) ==> (
+    match (sel h l) with
+    | LLNil -> True
+    | LLCons _ tl -> no_cycles_acc tl h (s `Set.union` !{l})
+  ))**)
+
+let rec footprint_fuel (fuel:nat) (ll:ref (linkedList int)) (h:heap) : GTot (Set.set nat) =
+  if fuel = 0 then Set.empty else (
+  !{ll} `Set.union` (
+    match sel h ll with
+    | LLNil -> Set.empty
+    | LLCons _ tl -> footprint_fuel (fuel-1) tl h)
+  )
 
 let rec refs_of_ll (fuel:nat) (ll:ref (linkedList int)) (h:heap) : GTot (list (ref (linkedList int))) =
   ll :: (
@@ -129,6 +265,23 @@ let rec label_llist_as_shareable_fuel (fuel:erased nat) (ll:ref (linkedList int)
   let h2 = get_heap () in
   assume (gets_shared (refs_of_ll_as_set fuel ll h2) h0 h2)
 
+let rec determine_fuel_fuel (ll:ref (linkedList int)) (ffuel:nat)
+  : SST (option nat)
+    (requires (fun h0 -> h0 `contains` ll))
+    (ensures (fun h0 ofuel h1 -> h0 == h1 /\ (Some? ofuel ==> (Some?.v ofuel <= ffuel) /\ no_cycles_fuel (Some?.v ofuel) ll h0)))
+    (decreases ffuel) =
+  if ffuel = 0 then None
+  else
+    match !ll with
+    | LLNil -> Some 1
+    | LLCons _ tl -> begin
+      let h0 = get_heap () in
+      eliminate_ctrans_ref_pred h0 #(SLList SNat) ll contains_pred;
+      match determine_fuel_fuel tl (ffuel-1) with
+      | None -> None
+      | Some fuel -> Some (fuel + 1)
+    end
+
 let label_llist_as_shareable (ll:ref (linkedList int)) (fuel:nat)
   : SST unit
     (requires (fun h0 -> h0 `contains` ll /\
@@ -190,54 +343,3 @@ let test1 () : STATEwp grade AllOps (fun _ _ -> False) =
   let gr : mref grade grade_preorder = alloc (NotGraded) in
  // auto_grader test solution gr;
   !gr
-
-let rec determine_fuel (ll:ref (linkedList int)) (ffuel:nat)
-  : SST (option nat)
-    (requires (fun h0 -> h0 `contains` ll))
-    (ensures (fun h0 ofuel h1 -> h0 == h1 /\ (Some? ofuel ==> (Some?.v ofuel <= ffuel) /\ no_cycles_fuel (Some?.v ofuel) ll h0)))
-    (decreases ffuel) =
-  if ffuel = 0 then None
-  else
-    match !ll with
-    | LLNil -> Some 1
-    | LLCons _ tl -> begin
-      let h0 = get_heap () in
-      eliminate_ctrans_ref_pred h0 #(SLList SNat) ll contains_pred;
-      match determine_fuel tl (ffuel-1) with
-      | None -> None
-      | Some fuel -> Some (fuel + 1)
-    end
-
-(**
-let same_elements (ll:ref (linkedList int)) (h0 h1:heap): Type0 =
-  let length_h0 = ll_length ll h0 in
-  let length_h1 = ll_length ll h1 in
-  if length_h0 <> length_h1 then False
-  else
-    exists fuel. elements_of_ll_acc fuel ll h0 FSet.emptyset == elements_of_ll_acc fuel ll h0 FSet.emptyset
-
- let same_elements_SST (ll: linkedList int): SST bool
-   (requires fun h0 -> satisfy_on_heap ll h0 contains_pred)
-   (ensures fun h0 r h1 -> r ==> same_elements ll h0 h1)
-   = admit()
-
-let rec sorted_SST (fuel: nat) (ll: linkedList int): SST bool
-  (requires fun h0 -> satisfy_on_heap ll h0 contains_pred)
-  (ensures fun h0 r h1 -> r ==> sorted ll h0) =
-  if fuel = 0 then false
-  else
-    match ll with
-    | LLNil -> true
-    | LLCons x next ->
-      let tl = sst_read next in
-      match tl with
-      | LLNil -> true
-      | LLCons y next ->
-        if x > y then false
-        else begin
-          let h = get_heap() in
-          heap_contains_all_refs_of_ll ll h;
-          admit();
-          sorted_SST (fuel - 1) tl
-        end
-**)
